build html

Term31.thy
@@ -6,7 +6,7 @@ chapter \<open>3.5 Evaluation\<close>
 
 section \<open>definition\<close>
 
-datatype t 
+datatype t
   = true
   | false
   | Cond t t t ("If _ Then _ Else _" [95,95,95] 90)
@@ -52,9 +52,9 @@ section \<open>3.5.4 deterministic of eval\<close>
 (* 3.5.4 *)
 theorem eval_deterministic: "\<lbrakk> t \<mapsto> t'; t \<mapsto> t'' \<rbrakk> \<Longrightarrow> t' = t''"
 proof(induct t arbitrary: t' t'')
-  case true thus ?case using true_cannot_eval by blast 
+  case true thus ?case using true_cannot_eval by blast
 next
-  case false thus ?case using false_cannot_eval by blast 
+  case false thus ?case using false_cannot_eval by blast
 next
   case Cond
   fix t1 t2 t3 t t''
@@ -75,7 +75,7 @@ next
   next
     case Cond
     obtain t1' where t1t1': "t1 \<mapsto> t1'" and t'if: "t' = (If t1' Then t2 Else t3)"
-      using Cond et' eval.cases by blast 
+      using Cond et' eval.cases by blast
     obtain t1'' where t1t1'': "t1 \<mapsto> t1''" and t''if: "t'' = (If t1'' Then t2 Else t3)"
       using Cond et'' eval.cases by blast
     have "t1' = t1''" using t1_induct t1t1' t1t1'' by simp
@@ -93,11 +93,11 @@ lemma is_normal_formI[elim]: "is_normal_form t \<Longrightarrow> \<not>(\<exists
 lemma true_is_normal_form[intro]: "is_normal_form true" using true_cannot_eval is_normal_form_def by simp
 lemma false_is_normal_form[intro]: "is_normal_form false" using false_cannot_eval is_normal_form_def by simp
 lemma normal_form_cannot_eval: "\<lbrakk> is_normal_form t; t \<mapsto> t' \<rbrakk> \<Longrightarrow> False" using is_normal_form_def by blast
-lemma if_isnot_normal_form: "\<not>(is_normal_form (If t1 Then t2 Else t3))"  
+lemma if_isnot_normal_form: "\<not>(is_normal_form (If t1 Then t2 Else t3))"
   apply (induct t1 arbitrary: t2 t3)
   using E_IfTrue is_normal_form_def apply blast
   using E_IfFalse is_normal_form_def apply blast
-  using E_If is_normal_form_def by metis 
+  using E_If is_normal_form_def by metis
 
 section \<open>3.5.7 value is normal form\<close>
 
@@ -169,7 +169,7 @@ lemma eval_star_deterministic: "\<lbrakk> t \<mapsto>* t'; is_normal_form t'; t 
 proof (induct rule: eval_star.induct)
   case (EsRefl t)
   then show ?case
-    using normal_form_cannot_eval by blast 
+    using normal_form_cannot_eval by blast
 next
   case (EsStep t t')
   then show ?case
@@ -185,21 +185,6 @@ inductive eval_n :: "t \<Rightarrow> nat \<Rightarrow> t \<Rightarrow> bool" ("_
   En0: "t \<mapsto>^0 t"
 | EnN: "\<lbrakk> t \<mapsto>^n t'; t' \<mapsto> t'' \<rbrakk> \<Longrightarrow> t \<mapsto>^(Suc n) t''"
 
-lemma exist_first_step: "\<lbrakk> t \<mapsto>^(Suc n) t' \<rbrakk> \<Longrightarrow> \<exists>t''. t \<mapsto>^n t'' \<and> t'' \<mapsto> t'"
-  by (metis eval_n.simps nat.inject old.nat.distinct(2))
-lemma exist_mid_step: "\<lbrakk> t \<mapsto>^(n + m) t' \<rbrakk> \<Longrightarrow> \<exists>t''. t \<mapsto>^n t'' \<and> t'' \<mapsto>^m t'"
-proof (induct m arbitrary: n t t')
-  case 0
-  then show ?case
-    using En0 by auto 
-next
-  case (Suc m)
-  then show ?case
-    by (metis EnN exist_first_step nat_arith.suc1) 
-qed
-lemma exist_mid_step2: "\<lbrakk> t \<mapsto>^n t'; m < n \<rbrakk> \<Longrightarrow> \<exists>t''. t \<mapsto>^m t'' \<and> t'' \<mapsto>^(n - m) t'"
-  using exist_mid_step by force
-
 lemma eval_0_refl[elim]: "t \<mapsto>^0 t' \<Longrightarrow> t = t'"
   by (metis Zero_neq_Suc eval_n.simps)
 lemma eval_1_step[elim]: "t \<mapsto>^1 t' \<Longrightarrow> t \<mapsto> t'"
@@ -210,15 +195,32 @@ proof (induct rule: eval_n.induct)
   then show ?case by (rule EsRefl)
 next
   case (EnN t t' n t'')
-  then show ?case by blast 
+  then show ?case by blast
 qed
+
+lemma exist_last_step: "\<lbrakk> t \<mapsto>^(Suc n) t' \<rbrakk> \<Longrightarrow> \<exists>t''. t \<mapsto>^n t'' \<and> t'' \<mapsto> t'"
+  by (metis eval_n.simps nat.inject old.nat.distinct(2))
+lemma exist_mid_step: "\<lbrakk> t \<mapsto>^(n + m) t' \<rbrakk> \<Longrightarrow> \<exists>t''. t \<mapsto>^n t'' \<and> t'' \<mapsto>^m t'"
+proof (induct m arbitrary: n t t')
+  case 0
+  then show ?case
+    using En0 by auto
+next
+  case (Suc m)
+  then show ?case
+    by (metis EnN exist_last_step nat_arith.suc1)
+qed
+lemma exist_mid_step2: "\<lbrakk> t \<mapsto>^n t'; m < n \<rbrakk> \<Longrightarrow> \<exists>t''. t \<mapsto>^m t'' \<and> t'' \<mapsto>^(n - m) t'"
+  using exist_mid_step by force
+lemma exist_first_step: "\<lbrakk> t \<mapsto>^(Suc n) t' \<rbrakk> \<Longrightarrow> \<exists>t''. t \<mapsto> t'' \<and> t'' \<mapsto>^n t'"
+  using exist_mid_step[where n=1, where m=n] by fastforce
 
 lemma eval_n_plus_1: "\<lbrakk> t \<mapsto>^n t'; t' \<mapsto> t'' \<rbrakk> \<Longrightarrow> t \<mapsto>^(Suc n) t''" by (simp add: EnN)
 lemma eval_n_plus_m: "\<lbrakk> t \<mapsto>^n t'; t' \<mapsto>^m t'' \<rbrakk> \<Longrightarrow> t \<mapsto>^(n+m) t''"
 proof (induct m arbitrary: n t t' t'')
   case 0
   then show ?case
-    using eval_0_refl by auto 
+    using eval_0_refl by auto
 next
   case (Suc n)
   then show ?case
@@ -235,15 +237,15 @@ lemma eval_star_eval_n[intro]: "t \<mapsto>* t' \<Longrightarrow> \<exists>n. t 
 proof (induct rule: eval_star.induct)
   case (EsRefl t)
   then show ?case
-    using En0 by blast 
+    using En0 by blast
 next
   case (EsStep t t')
   then show ?case
-    using step_eval_1 by blast 
+    using step_eval_1 by blast
 next
   case (EsTrans t t' t'')
   then show ?case
-    using eval_n_plus_m by blast 
+    using eval_n_plus_m by blast
 qed
 
 lemma can_eval_suc_inot_normal_form: "\<lbrakk> t \<mapsto>^n t'; n > 0 \<rbrakk> \<Longrightarrow> \<not>(is_normal_form t)"
@@ -255,13 +257,13 @@ theorem eval_n_deterministic: "\<lbrakk> t \<mapsto>^n t'; t \<mapsto>^n t'' \<r
 proof (induct n arbitrary: t t' t'')
   case 0
   then show ?case
-    using eval_0_refl by blast 
+    using eval_0_refl by blast
 next
   case (Suc n)
   assume "t \<mapsto>^(Suc n) t'"
-  with exist_first_step obtain tp' where tp'n:"t \<mapsto>^n tp'" and tp'next:"tp' \<mapsto> t'" by blast
+  with exist_last_step obtain tp' where tp'n:"t \<mapsto>^n tp'" and tp'next:"tp' \<mapsto> t'" by blast
   assume "t \<mapsto>^(Suc n) t''"
-  with exist_first_step obtain tp'' where tp''n:"t \<mapsto>^n tp''" and tp''next:"tp'' \<mapsto> t''" by blast
+  with exist_last_step obtain tp'' where tp''n:"t \<mapsto>^n tp''" and tp''next:"tp'' \<mapsto> t''" by blast
   have eq:"tp' = tp''" using tp'n tp''n Suc(1) by blast
   show "t' = t''"
     using tp'next tp''next eq eval_deterministic by simp
@@ -331,7 +333,7 @@ qed
 theorem eval_star_stop: "\<exists>t'. t \<mapsto>* t' \<and> is_normal_form t'"
 proof (induct t)
   case true
-  then show ?case by blast 
+  then show ?case by blast
 next
   case false
   then show ?case by blast
@@ -341,8 +343,220 @@ next
   hence t1_true_false: "t1' = true \<or> t1' = false" using normal_form_is_value is_value_def by simp
   hence "If t1 Then t2 Else t3 \<mapsto>* t2 \<or> If t1 Then t2 Else t3 \<mapsto>* t3"
     using eval_star_IfTrue eval_star_IfFalse t1t1' by blast
-  with Cond.hyps(2) Cond.hyps(3) eval_star_trans3 
+  with Cond.hyps(2) Cond.hyps(3) eval_star_trans3
   show "\<exists>t'. If t1 Then t2 Else t3 \<mapsto>* t' \<and> is_normal_form t'" by blast
+qed
+
+
+section \<open>3.5.13 (1)\<close>
+
+inductive eval_funny1 :: "t \<Rightarrow> t \<Rightarrow>  bool" ("_ \<mapsto>f1 _" [50,50] 40)
+  where
+    E_IfTrueF1: "If true Then t2 Else t3 \<mapsto>f1 t2"
+  | E_IfFalseF1: "If false Then t2 Else t3 \<mapsto>f1 t3"
+  | E_IfF1:  "t1 \<mapsto>f1 t1' \<Longrightarrow> If t1 Then t2 Else t3 \<mapsto>f1 If t1' Then t2 Else t3"
+  | E_Funny1: "If true Then t2 Else t3 \<mapsto>f1 t3"
+
+definition is_normal_form_f1 :: "t \<Rightarrow> bool"
+  where "is_normal_form_f1 t \<longleftrightarrow> \<not>(\<exists>t'. t \<mapsto>f1 t')"
+
+inductive eval_star_f1 :: "t \<Rightarrow> t \<Rightarrow> bool" ("_ \<mapsto>f1* _" [50,50] 40) where
+    EsReflF1: "t \<mapsto>f1* t"
+  | EsStepF1: "\<lbrakk> t \<mapsto>f1 t' \<rbrakk> \<Longrightarrow> t \<mapsto>f1* t'"
+  | EsTransF1: "\<lbrakk> t \<mapsto>f1* t'; t' \<mapsto>f1* t'' \<rbrakk> \<Longrightarrow> t \<mapsto>f1* t''"
+
+subsection \<open>lemmas\<close>
+
+lemma eval_funny1_is_eval: "t \<mapsto> t' \<Longrightarrow> t \<mapsto>f1 t'"
+  by (simp add: E_IfF1 E_IfFalseF1 E_IfTrueF1 eval.inducts)
+
+
+lemma is_normal_f1_formE[intro]: "\<not>(\<exists>t'. t \<mapsto>f1 t') \<Longrightarrow> is_normal_form_f1 t" using is_normal_form_f1_def by simp
+lemma is_normal_f1_formI[elim]: "is_normal_form_f1 t \<Longrightarrow> \<not>(\<exists>t'. t \<mapsto>f1 t')" using is_normal_form_f1_def by simp
+
+lemma true_is_normal_form_f1[intro]: "is_normal_form_f1 true" using eval_funny1.cases by blast
+lemma false_is_normal_form_f1[intro]: "is_normal_form_f1 false" using eval_funny1.cases by blast
+lemma normal_form_f1_cannot_eval: "\<lbrakk> is_normal_form_f1 t; t \<mapsto>f1 t' \<rbrakk> \<Longrightarrow> False" using eval_funny1_is_eval is_normal_f1_formI by blast
+lemma if_isnot_normal_form_f1: "\<not>(is_normal_form_f1 (If t1 Then t2 Else t3))" using eval_funny1_is_eval if_isnot_normal_form normal_form_f1_cannot_eval by blast
+
+lemma eval_star_f1_refl[intro]: "t = t' \<Longrightarrow> t \<mapsto>f1* t'" using EsReflF1 by simp
+lemma eval_star_f1_step[intro]: "t \<mapsto>f1 t' \<Longrightarrow> t \<mapsto>f1* t'" by (rule EsStepF1)
+lemma eval_star_f1_trans1[intro]: "\<lbrakk> t \<mapsto>f1* t'; t' \<mapsto>f1* t'' \<rbrakk> \<Longrightarrow> t \<mapsto>f1* t''" by (rule EsTransF1)
+lemma eval_star_f1_trans2[intro]: "\<lbrakk> t \<mapsto>f1 t'; t' \<mapsto>f1* t'' \<rbrakk>  \<Longrightarrow> t \<mapsto>f1* t''" using EsStepF1 EsTransF1 by blast
+lemma eval_star_f1_trans3[intro]: "\<lbrakk> t \<mapsto>f1* t'; t' \<mapsto>f1 t'' \<rbrakk>  \<Longrightarrow> t \<mapsto>f1* t''" using EsStepF1 EsTransF1 by blast
+
+lemma E_If_star_f1: "t1 \<mapsto>f1* t1' \<Longrightarrow> If t1 Then t2 Else t3 \<mapsto>f1* If t1' Then t2 Else t3"
+proof (induct rule: eval_star_f1.induct)
+  case (EsReflF1 t)
+  then show ?case by force
+next
+  case (EsStepF1 t t')
+  show ?case by (simp add: E_IfF1 eval_star_f1_step local.EsStepF1)
+next
+  case (EsTransF1 t t' t'')
+  show ?case using EsTransF1.hyps(2) EsTransF1.hyps(4) by blast
+qed
+
+lemma eval_star_f1_IfTrue: "\<lbrakk> t1 \<mapsto>f1* true \<rbrakk> \<Longrightarrow> If t1 Then t2 Else t3 \<mapsto>f1* t2"
+  using E_If_star_f1[of t1, of true] E_IfTrueF1 eval_star_f1_trans2 eval_star_f1_trans3 by blast
+
+lemma eval_star_f1_IfFalse: "\<lbrakk> t1 \<mapsto>f1* false \<rbrakk> \<Longrightarrow> If t1 Then t2 Else t3 \<mapsto>f1* t3"
+  using E_If_star_f1[of t1, of false] E_IfFalseF1 eval_star_f1_trans2 eval_star_f1_trans3 by blast
+
+subsection \<open>proofs\<close>
+
+(* 3.5.4 *)
+theorem eval_deterministic_f1: "\<lbrakk> t \<mapsto>f1 t'; t \<mapsto>f1 t'' \<rbrakk> \<Longrightarrow> t' = t''"
+  nitpick
+  oops
+theorem eval_deterministic_f1_not: "\<exists>t t' t''. \<not>((t \<mapsto>f1 t' \<and> t \<mapsto>f1 t'') \<longrightarrow> t' = t'')"
+  apply (rule exI[where x="If true Then true Else (If true Then true Else true)"])
+  apply (rule exI[where x="If true Then true Else true"])
+  apply (rule exI[where x="true"])
+  by (simp add: E_Funny1 E_IfTrueF1)
+
+(* 3.5.7 *)
+theorem value_is_normal_form_f1: "is_value t \<Longrightarrow> is_normal_form_f1 t"
+  using is_value_def by fastforce
+
+(* 3.5.8 *)
+theorem normal_form_f1_is_value: "is_normal_form_f1 t \<Longrightarrow> is_value t"
+  apply (rule t.exhaust[of t], blast, blast)
+  apply (simp add: if_isnot_normal_form_f1)
+  done
+
+(* 3.5.11 *)
+lemma eval_star_deterministic_f1: "\<lbrakk> t \<mapsto>f1* t'; is_normal_form_f1 t'; t \<mapsto>f1* t''; is_normal_form_f1 t'' \<rbrakk> \<Longrightarrow> t' = t''"
+  nitpick
+  oops
+theorem eval_star_deterministic_f1_not: "\<exists>t t' t''. \<not>((t \<mapsto>f1* t' \<and> is_normal_form_f1 t' \<and> t \<mapsto>f1* t'' \<and> is_normal_form_f1 t'') \<longrightarrow> t' = t'')"
+  apply (rule exI[where x="If true Then true Else false"])
+  apply (rule exI[where x="false"])
+  apply (rule exI[where x="true"])
+  using E_Funny1 E_IfTrueF1 eval_star_f1_step false_is_normal_form_f1 t.distinct(1) true_is_normal_form_f1 by presburger
+
+(* 3.5.12 *)
+theorem eval_star_f1_stop: "\<exists>t'. t \<mapsto>f1* t' \<and> is_normal_form_f1 t'"
+proof (induct t)
+  case true
+  then show ?case
+    using EsReflF1 by blast
+next
+  case false
+  then show ?case
+    using EsReflF1 by blast
+next
+  case (Cond t1 t2 t3)
+  obtain t1' where t1t1': "t1 \<mapsto>f1* t1'" and "is_normal_form_f1 t1'" using Cond.hyps(1) by blast
+  hence t1_true_false: "t1' = true \<or> t1' = false" using normal_form_f1_is_value is_value_def by simp
+  hence "If t1 Then t2 Else t3 \<mapsto>f1* t2 \<or> If t1 Then t2 Else t3 \<mapsto>f1* t3"
+    using eval_star_f1_IfTrue eval_star_f1_IfFalse t1t1' by blast
+  with Cond.hyps(2) Cond.hyps(3) eval_star_trans3
+  show "\<exists>t'. If t1 Then t2 Else t3 \<mapsto>f1* t' \<and> is_normal_form_f1 t'" by blast
+qed
+
+
+section \<open>3.5.13 (2)\<close>
+
+inductive eval_funny2 :: "t \<Rightarrow> t \<Rightarrow>  bool" ("_ \<mapsto>f2 _" [50,50] 40)
+  where
+    E_IfTrueF2: "If true Then t2 Else t3 \<mapsto>f2 t2"
+  | E_IfFalseF2: "If false Then t2 Else t3 \<mapsto>f2 t3"
+  | E_IfF2:  "t1 \<mapsto>f2 t1' \<Longrightarrow> If t1 Then t2 Else t3 \<mapsto>f2 If t1' Then t2 Else t3"
+  | E_Funny2: "t2 \<mapsto>f2 t2' \<Longrightarrow> If true Then t2 Else t3 \<mapsto>f2 If true Then t2' Else t3"
+
+definition is_normal_form_f2 :: "t \<Rightarrow> bool"
+  where "is_normal_form_f2 t \<longleftrightarrow> \<not>(\<exists>t'. t \<mapsto>f2 t')"
+
+inductive eval_star_f2 :: "t \<Rightarrow> t \<Rightarrow> bool" ("_ \<mapsto>f2* _" [50,50] 40) where
+    EsReflF2: "t \<mapsto>f2* t"
+  | EsStepF2: "\<lbrakk> t \<mapsto>f2 t' \<rbrakk> \<Longrightarrow> t \<mapsto>f2* t'"
+  | EsTransF2: "\<lbrakk> t \<mapsto>f2* t'; t' \<mapsto>f2* t'' \<rbrakk> \<Longrightarrow> t \<mapsto>f2* t''"
+
+subsection \<open>lemmas\<close>
+
+lemma eval_funny2_is_eval: "t \<mapsto> t' \<Longrightarrow> t \<mapsto>f2 t'"
+  by (simp add: E_IfF2 E_IfFalseF2 E_IfTrueF2 eval.inducts)
+
+
+lemma is_normal_f2_formE[intro]: "\<not>(\<exists>t'. t \<mapsto>f2 t') \<Longrightarrow> is_normal_form_f2 t" using is_normal_form_f2_def by simp
+lemma is_normal_f2_formI[elim]: "is_normal_form_f2 t \<Longrightarrow> \<not>(\<exists>t'. t \<mapsto>f2 t')" using is_normal_form_f2_def by simp
+
+lemma true_is_normal_form_f2[intro]: "is_normal_form_f2 true" using eval_funny2.cases by blast
+lemma false_is_normal_form_f2[intro]: "is_normal_form_f2 false" using eval_funny2.cases by blast
+lemma normal_form_f2_cannot_eval: "\<lbrakk> is_normal_form_f2 t; t \<mapsto>f2 t' \<rbrakk> \<Longrightarrow> False" using eval_funny2_is_eval is_normal_f2_formI by blast
+lemma if_isnot_normal_form_f2: "\<not>(is_normal_form_f2 (If t1 Then t2 Else t3))" using eval_funny2_is_eval if_isnot_normal_form normal_form_f2_cannot_eval by blast
+
+lemma eval_star_f2_refl[intro]: "t = t' \<Longrightarrow> t \<mapsto>f2* t'" using EsReflF2 by simp
+lemma eval_star_f2_step[intro]: "t \<mapsto>f2 t' \<Longrightarrow> t \<mapsto>f2* t'" by (rule EsStepF2)
+lemma eval_star_f2_trans1[intro]: "\<lbrakk> t \<mapsto>f2* t'; t' \<mapsto>f2* t'' \<rbrakk> \<Longrightarrow> t \<mapsto>f2* t''" by (rule EsTransF2)
+lemma eval_star_f2_trans2[intro]: "\<lbrakk> t \<mapsto>f2 t'; t' \<mapsto>f2* t'' \<rbrakk>  \<Longrightarrow> t \<mapsto>f2* t''" using EsStepF2 EsTransF2 by blast
+lemma eval_star_f2_trans3[intro]: "\<lbrakk> t \<mapsto>f2* t'; t' \<mapsto>f2 t'' \<rbrakk>  \<Longrightarrow> t \<mapsto>f2* t''" using EsStepF2 EsTransF2 by blast
+
+lemma E_If_star_f2: "t1 \<mapsto>f2* t1' \<Longrightarrow> If t1 Then t2 Else t3 \<mapsto>f2* If t1' Then t2 Else t3"
+proof (induct rule: eval_star_f2.induct)
+  case (EsReflF2 t)
+  then show ?case by force
+next
+  case (EsStepF2 t t')
+  show ?case by (simp add: E_IfF2 eval_star_f2_step local.EsStepF2)
+next
+  case (EsTransF2 t t' t'')
+  show ?case using EsTransF2.hyps(2) EsTransF2.hyps(4) by blast
+qed
+
+lemma eval_star_f2_IfTrue: "\<lbrakk> t1 \<mapsto>f2* true \<rbrakk> \<Longrightarrow> If t1 Then t2 Else t3 \<mapsto>f2* t2"
+  using E_If_star_f2[of t1, of true] E_IfTrueF2 eval_star_f2_trans2 eval_star_f2_trans3 by blast
+
+lemma eval_star_f2_IfFalse: "\<lbrakk> t1 \<mapsto>f2* false \<rbrakk> \<Longrightarrow> If t1 Then t2 Else t3 \<mapsto>f2* t3"
+  using E_If_star_f2[of t1, of false] E_IfFalseF2 eval_star_f2_trans2 eval_star_f2_trans3 by blast
+
+subsection \<open>proofs\<close>
+
+(* 3.5.4 *)
+theorem eval_deterministic_f2: "\<lbrakk> t \<mapsto>f2 t'; t \<mapsto>f2 t'' \<rbrakk> \<Longrightarrow> t' = t''"
+  nitpick
+  oops
+theorem eval_deterministic_f2_not: "\<exists>t t' t''. \<not>((t \<mapsto>f2 t' \<and> t \<mapsto>f2 t'') \<longrightarrow> t' = t'')"
+  apply (rule exI[where x="If true Then (If true Then true Else true) Else (If true Then true Else true)"])
+  apply (rule exI[where x="If true Then true Else true"])
+  apply (rule exI[where x="If true Then true Else (If true Then true Else true)"])
+  by (simp add: E_Funny2 E_IfTrueF2)
+
+
+(* 3.5.7 *)
+theorem value_is_normal_form_f2: "is_value t \<Longrightarrow> is_normal_form_f2 t"
+  using is_value_def by fastforce
+
+(* 3.5.8 *)
+theorem normal_form_f2_is_value: "is_normal_form_f2 t \<Longrightarrow> is_value t"
+  apply (rule t.exhaust[of t], blast, blast)
+  apply (simp add: if_isnot_normal_form_f2)
+  done
+
+(* 3.5.11 *)
+lemma eval_star_deterministic_f2: "\<lbrakk> t \<mapsto>f2* t'; is_normal_form_f2 t'; t \<mapsto>f2 t''; is_normal_form_f2 t'' \<rbrakk> \<Longrightarrow> t' = t''"
+(* proof should be changed *)
+  oops
+
+(* 3.5.12 *)
+theorem eval_star_f2_stop: "\<exists>t'. t \<mapsto>f2* t' \<and> is_normal_form_f2 t'"
+proof (induct t)
+  case true
+  then show ?case
+    using EsReflF2 by blast
+next
+  case false
+  then show ?case
+    using EsReflF2 by blast
+next
+  case (Cond t1 t2 t3)
+  obtain t1' where t1t1': "t1 \<mapsto>f2* t1'" and "is_normal_form_f2 t1'" using Cond.hyps(1) by blast
+  hence t1_true_false: "t1' = true \<or> t1' = false" using normal_form_f2_is_value is_value_def by simp
+  hence "If t1 Then t2 Else t3 \<mapsto>f2* t2 \<or> If t1 Then t2 Else t3 \<mapsto>f2* t3"
+    using eval_star_f2_IfTrue eval_star_f2_IfFalse t1t1' by blast
+  with Cond.hyps(2) Cond.hyps(3) eval_star_trans3
+  show "\<exists>t'. If t1 Then t2 Else t3 \<mapsto>f2* t' \<and> is_normal_form_f2 t'" by blast
 qed
 
 end
