Makefile
@@ -1,0 +1,10 @@
+.PHONY: presentation
+presentation:
+	isabelle build -o browser_info -P build -v -d . tapl-isabelle
+	mkdir -p presentation presentation/fonts
+	mv build/fonts/* presentation/fonts/
+	mv build/Unsorted/tapl-isabelle/* presentation/
+	sed "s_url('\.\./\.\./fonts/_url('fonts/_" -i presentation/isabelle.css
+	rm presentation/session_graph.pdf
+	rm presentation/index.html
+	rm -rf build
